SKI.Equality.fst
@@ -4,14 +4,7 @@ open SKI
 open Subst
 
 
-type ski_step : ski -> ski -> Type =
-  | Red_S : f : ski -> g : ski -> x : ski ->
-            ski_step (App (App (App S f) g) x) (App (App f x) (App g x))
-  | Red_K : a : ski -> b : ski ->
-            ski_step (App (App K a) b) a
-  | Red_I : x : ski -> ski_step (App I x) x
-
-let fnl (t : ski) : bool = match t with
+let fnl (t : term) : bool = match t with
   | App (App S _) _ -> true
   | App S _ -> true
   | App K _ -> true
@@ -20,25 +13,50 @@ let fnl (t : ski) : bool = match t with
   | I -> true
   | _ -> false
 
+
+let rel (a b : Type) = a -> b -> Type
+
+noeq
+type eq (#a : Type) (app : a -> a -> a) (r : rel a a)
+: a -> a -> Type =
+  | Refl : t : a -> eq app r t t
+  | Symm : #t : a -> #u : a -> r t u -> eq app r u t
+  | Tran : #t : a -> #u : a -> #v : a ->
+            r t u -> r u v -> eq app r t v
+  | AppL : #t : a -> #t' : a ->
+            r t t' -> u : a ->
+            eq app r (app t u) (app t' u)
+  | AppR : t : a -> #u : a -> #u' : a ->
+            r u u' -> eq app r (app t u) (app t u')
+
+
+let lapp (x y : lam) : z : lam {z = App x y} = App x y
+
+noeq
+type lam_eq : lam -> lam -> Type =
+  | Beta : t : lam -> u : lam -> lam_eq (App (Abs t) u) (subst0 t u)
+  | Down : #t : lam -> #t' : lam -> lam_eq t t' -> lam_eq (Abs t) (Abs t') 
+  | Eq_L : #t : lam -> #u : lam -> eq lapp lam_eq t u -> lam_eq t u 
+
+
+let sapp (x y : ski) : z : ski {z = App x y} = App x y
+
 noeq
 type ski_eq : ski -> ski -> Type =
-  | SRefl : t : ski -> ski_eq t t
-  | SSymm : #t : ski -> #u : ski -> ski_eq t u -> ski_eq u t
-  | STran : #t : ski -> #u : ski -> #v : ski ->
-            ski_eq t u -> ski_eq u v -> ski_eq t v
-  // voy a tener q cambiar esto y tener AppL y AppR
-  | SAppL : #t : ski -> #t' : ski ->
-            ski_eq t t' -> u : ski ->
-            ski_eq (App t u) (App t' u)
-  | SAppR : t : ski -> #u : ski -> #u' : ski ->
-            ski_eq u u' -> ski_eq (App t u) (App t u')
+  | RedS : f : ski -> g : ski -> x : ski ->
+            ski_eq (App (App (App S f) g) x) (App (App f x) (App g x))
+  | RedK : a : ski -> b : ski ->
+            ski_eq (App (App K a) b) a
+  | RedI : x : ski -> ski_eq (App I x) x
   | Zeta : #t : ski {fnl t} -> #u : ski {fnl u} ->
            (i : nat {not_free i t && not_free i u} ->
            ski_eq (App t (Var i)) (App u (Var i))) ->
            ski_eq t u
-  | SStep : #t : ski -> #u : ski -> ski_step t u -> ski_eq t u
+  | Eq_S : #t : ski -> #u : ski -> eq sapp ski_eq t u -> ski_eq t u
 
-let ski_app_eq (#t #t' #u #u' : ski)
-               (eq_t : ski_eq t t') (eq_u : ski_eq u u')
-: ski_eq (App t u) (App t' u')
-= STran (SAppL eq_t u) (SAppR t' eq_u)
+
+
+let app_eq_ski (#t #t' #u #u' : ski)
+           (eq_t : ski_eq t t') (eq_u : ski_eq u u')
+: (if true then ski_eq else ski_eq) (App t u) (App t' u')
+= Eq_S (Tran (Eq_S (AppL eq_t u)) (Eq_S (AppR t' #u #u' eq_u)))
