BracketAbstraction.Equality.fst
@@ -4,9 +4,6 @@ open SKI
 open SKI.Equality 
 open BracketAbstraction
 open Subst
-open Lam.Equality
-
-
 
 let rec abstract_App (t v : ski)
 : ski_eq (App (abstract t) v) (subst_ski t v 0)
@@ -14,41 +11,33 @@ let rec abstract_App (t v : ski)
   | App t u ->
     let abs_t = abstract t  in
     let abs_u = abstract u  in
-    let red_s = SStep (Red_S abs_t abs_u v) in
+    let red_s = RedS abs_t abs_u v in
     let hi_t = abstract_App t v in
     let hi_u = abstract_App u v in
-    let app_eq = ski_app_eq hi_t hi_u in
-    STran red_s app_eq
-  | Var 0 -> SStep (Red_I v)
-  | Var j -> SStep (Red_K (Var (j - 1)) v)
-  | S -> SStep (Red_K S v)
-  | K -> SStep (Red_K K v)
-  | I -> SStep (Red_K I v)
-  | Unit -> SStep (Red_K Unit v)
+    let app_eq = app_eq_ski hi_t hi_u in
+    Eq_S (Tran red_s app_eq)
+  | Var 0 -> RedI v
+  | Var j -> RedK (Var (j - 1)) v
+  | S -> RedK S v
+  | K -> RedK K v
+  | I -> RedK I v
+  | Unit -> RedK Unit v
 
 
-let subst_ski_step_eq (#t #u: ski) (st : ski_step t u)
-                      (v : ski)
-: Tot (ski_eq (subst_ski t v 0) (subst_ski u v 0))
-      (decreases st)
-= let sub t = subst_ski t v 0 in
-  match st with
-  | Red_S f g x -> SStep (Red_S (sub f) (sub g) (sub x))
-  | Red_K x y -> SStep (Red_K (sub x) (sub y))
-  | Red_I x -> SStep (Red_I (sub x))
-
-let rec subst_ski_eq (#t #u: ski) (eq : ski_eq t u)
+let rec subst_ski_eq (#t #u: ski) (r : ski_eq t u)
                      (v : ski)
 : Tot (ski_eq (subst_ski t v 0) (subst_ski u v 0))
-      (decreases eq)
+      (decreases r)
 = let sub t = subst_ski t v 0 in
-  match eq with
-  | SRefl _ -> SRefl _
-  | SSymm eq -> SSymm (subst_ski_eq eq v)
-  | STran eq1 eq2 -> STran (subst_ski_eq eq1 v) (subst_ski_eq eq2 v)
-  // | ski_app_eq eq1 eq2 -> ski_app_eq (subst_ski_eq eq1 v) (subst_ski_eq eq2 v)
-  | SAppL eq u -> SAppL (subst_ski_eq eq v) (subst_ski u v 0)
-  | SAppR t eq -> SAppR (subst_ski t v 0) (subst_ski_eq eq v)
+  match r with
+  | Eq_S (Refl _) -> Eq_S (Refl _)
+  | Eq_S (Symm r) -> Eq_S (Symm (subst_ski_eq r v))
+  | Eq_S (Tran eq1 eq2) -> Eq_S (Tran (subst_ski_eq eq1 v) (subst_ski_eq eq2 v))
+  | Eq_S (AppL r u) -> Eq_S (AppL (subst_ski_eq r v) (subst_ski u v 0))
+  | Eq_S (AppR t r) -> Eq_S (AppR (subst_ski t v 0) (subst_ski_eq r v))
+  | RedS f g x -> RedS (sub f) (sub g) (sub x)
+  | RedK x y -> RedK (sub x) (sub y)
+  | RedI x -> RedI (sub x)
   | Zeta ext ->
     let t' = subst_ski t v 0 in
     let u' = subst_ski u v 0 in
@@ -58,7 +47,6 @@ let rec subst_ski_eq (#t #u: ski) (eq : ski_eq t u)
       not_free_subst_ski u v i ;
       subst_ski_eq (ext (i + 1)) v in
     Zeta ext'
-  | SStep st -> subst_ski_step_eq st v
 
 let app2 (t u v : ski) : ski = App (App t u) v
 let app3 (t u v w : ski) : ski = App (app2 t u v) w
@@ -68,85 +56,81 @@ let ( @ ) (t u : ski) : ski = App t u
 let abstract_S_ski_eq (f g x y : ski)
 : ski_eq (((S @ ((S @ ((S @ (K @ S)) @ f)) @ g)) @ x) @ y)
          (((S @ ((S @ f) @ x)) @ ((S @ g) @ x)) @ y)
-= let red_1 = Red_S ((S  @ ((S @ (K @ S)) @ f)) @ g) x y in
-  let red_2 = Red_S (App (App S (App K S)) f) g y in
-  let red_2 = Red_S ((S @ (K @ S)) @ f) g y in
-  let red_3 = Red_S (K @ S) f y in
-  let red_4 = Red_K S y in
-  let app_2 = SAppL (SStep red_2) (x @ y) in
-  let app_3_1 = SAppL (SStep red_3) (g @ y) in
-  let app_3_2 = SAppL app_3_1 (x @ y) in
-  let app_4_1 = SAppL (SStep red_4) (f @ y) in
-  let app_4_2 = SAppL app_4_1 (g @ y) in 
-  let app_4_3 = SAppL app_4_2 (x @ y) in
-  let red_5 = Red_S (f @ y) (g @ y) (x @ y) in
-  let lhs = STran (SStep red_1) app_2 in
-  let lhs = STran lhs app_3_2 in
-  let lhs = STran lhs app_4_3 in
-  let lhs = STran lhs (SStep red_5) in
-  let red_1 = Red_S ((S @ f) @ x) ((S @ g) @ x) y in
-  let redl = Red_S f x y in
-  let redr = Red_S g x y in
-  let app = ski_app_eq (SStep redl) (SStep redr) in
-  let rhs = STran (SStep red_1) app in
-  STran lhs (SSymm rhs)
+= let k : ski = ((S @ ((S @ (K @ S)) @ f)) @ g) in
+  let red_1 = RedS k x y in
+  let red_2 = RedS (App (App S (App K S)) f) g y in
+  let red_2 = RedS ((S @ (K @ S)) @ f) g y in
+  let red_3 = RedS (K @ S) f y in
+  let red_4 = RedK S y in
+  let app_2 = Eq_S (AppL red_2 (x @ y)) in
+  let app_3_1 = Eq_S (AppL red_3 (g @ y)) in
+  let app_3_2 = Eq_S (AppL app_3_1 (x @ y)) in
+  let app_4_1 = Eq_S (AppL red_4 (f @ y)) in
+  let app_4_2 = Eq_S (AppL app_4_1 (g @ y)) in 
+  let app_4_3 = Eq_S (AppL app_4_2 (x @ y)) in
+  let red_5 = RedS (f @ y) (g @ y) (x @ y) in
+  let lhs = Eq_S (Tran red_1 app_2) in
+  let lhs = Eq_S (Tran lhs app_3_2) in
+  let lhs = Eq_S (Tran lhs app_4_3) in
+  let lhs = Eq_S (Tran lhs red_5) in
+  let red_1 = RedS ((S @ f) @ x) ((S @ g) @ x) y in
+  let redl = RedS f x y in
+  let redr = RedS g x y in
+  let app = app_eq_ski redl redr in
+  let rhs = Eq_S (Tran red_1 app) in
+  Eq_S (Tran lhs (Eq_S (Symm rhs)))
 
 let abstract_K_ski_eq (x y z : ski)
 : ski_eq (((S @ ((S @ (K @ K)) @ x)) @ y) @ z)
          (x @ z)
-= let red_S_1 = Red_S ((S @ (K @ K)) @ x) y z in
-  let red_S_2 = Red_S (K @ K) x z in
-  let red_K_1 = Red_K K z in
-  let red_K_2 = Red_K (x @ z) (y @ z) in
-  let app_1 = SAppL (SStep red_S_2) (y @ z) in
-  let app_2 = SAppL (SAppL (SStep red_K_1) _) _ in
-  let lhs_1 = STran (SStep red_S_1) app_1 in
-  let lhs_2 = STran lhs_1 app_2 in
-  STran lhs_2 (SStep red_K_2)
+= let red_S_1 = RedS ((S @ (K @ K)) @ x) y z in
+  let red_S_2 = RedS (K @ K) x z in
+  let red_K_1 = RedK K z in
+  let red_K_2 = RedK (x @ z) (y @ z) in
+  let app_1 = Eq_S (AppL red_S_2 (y @ z)) in
+  let app_2 = Eq_S (AppL (Eq_S (AppL red_K_1 _)) _) in
+  let lhs_1 = Eq_S (Tran red_S_1 app_1) in
+  let lhs_2 = Eq_S (Tran lhs_1 app_2) in
+  Eq_S (Tran lhs_2 red_K_2)
 
 let abstract_I_ski_eq (x y : ski)
 : ski_eq (((S @ (K @ I)) @ x) @ y)
          (x @ y)
-= let red_S = Red_S (K @ I) x y in
-  let red_K = Red_K I y in
-  let red_I = Red_I (x @ y) in
-  let app = SAppL (SStep red_K) _ in
-  STran (STran (SStep red_S) app) (SStep red_I)
+= let red_S = RedS (K @ I) x y in
+  let red_K = RedK I y in
+  let red_I = RedI (x @ y) in
+  let app = Eq_S (AppL red_K _) in
+  Eq_S (Tran (Eq_S (Tran red_S app)) red_I)
 
-let abstract_ski_step_eq (#t #u : ski) (st : ski_step t u)
-: Tot (ski_eq (abstract t) (abstract u))
-      (decreases st)
-= match st with
-| Red_S f g x ->
-  let f' : ski= abstract f in
-  let g' : ski= abstract g in
-  let x' : ski= abstract x in
-  let ext (i : nat {not_free i f' && not_free i g' && not_free i x'})
-  = abstract_S_ski_eq f' g' x' (Var i)
-  in Zeta ext
-| Red_K x y ->
-  let x' : ski = abstract x in
-  let y' : ski = abstract y in
-  let ext (i : nat {not_free i x' && not_free i y'})
-  = abstract_K_ski_eq x' y' (Var i)
-  in Zeta ext
-| Red_I x ->
-let x' : ski = abstract x in
-let ext (i : nat {not_free i x'})
-= abstract_I_ski_eq x' (Var i)
-in Zeta ext
 
 
 let rec abstract_ski_eq (#t #u : ski) (t_eq_u : ski_eq t u)
 : Tot (ski_eq (abstract t) (abstract u))
       (decreases t_eq_u)
 = match t_eq_u with
-| SRefl t -> SRefl _
-| SSymm eq -> SSymm (abstract_ski_eq eq)
-| STran eq1 eq2 -> STran (abstract_ski_eq eq1) (abstract_ski_eq eq2)
-// | ski_app_eq eq1 eq2 -> ski_app_eq (ski_app_eq (SRefl S) (abstract_ski_eq eq1)) (abstract_ski_eq eq2)
-| SAppL eq u -> SAppL (SAppR S (abstract_ski_eq eq)) (abstract u) 
-| SAppR t eq -> SAppR (App S (abstract t)) (abstract_ski_eq eq)
+| Eq_S (Refl t) -> Eq_S (Refl _)
+| Eq_S (Symm r) -> Eq_S (Symm (abstract_ski_eq r))
+| Eq_S (Tran eq1 eq2) -> Eq_S (Tran (abstract_ski_eq eq1) (abstract_ski_eq eq2))
+| Eq_S (AppL r u) -> Eq_S (AppL (Eq_S (AppR S (abstract_ski_eq r))) (abstract u)) 
+| Eq_S (AppR t r) -> Eq_S (AppR (App S (abstract t)) (abstract_ski_eq r))
+| RedS f g x ->
+  let f' : ski= abstract f in
+  let g' : ski= abstract g in
+  let x' : ski= abstract x in
+  let ext (i : nat {not_free i f' && not_free i g' && not_free i x'})
+  = abstract_S_ski_eq f' g' x' (Var i)
+  in Zeta ext
+| RedK x y ->
+  let x' : ski = abstract x in
+  let y' : ski = abstract y in
+  let ext (i : nat {not_free i x' && not_free i y'})
+  = abstract_K_ski_eq x' y' (Var i)
+  in Zeta ext
+| RedI x ->
+  let x' : ski = abstract x in
+  let ext (i : nat {not_free i x'})
+  = abstract_I_ski_eq x' (Var i)
+  in Zeta ext
 | Zeta ext ->
   let t' = abstract t in
   let u' = abstract u in
@@ -160,9 +144,8 @@ let rec abstract_ski_eq (#t #u : ski) (t_eq_u : ski_eq t u)
     = not_free_subst_ski t (Var i) j ; 
       not_free_subst_ski u (Var i) j ;
       subst_ski_eq (ext (j + 1)) (Var i)
-    in STran (STran abs_app_t (Zeta ext'')) (SSymm abs_app_u)
+    in Eq_S (Tran (Eq_S (Tran abs_app_t (Zeta ext''))) (Eq_S (Symm abs_app_u)))
   in Zeta ext'
-| SStep st -> abstract_ski_step_eq st
 
 
 
@@ -176,7 +159,7 @@ let rec shift_bracket (i : nat) (t : lam)
 : Lemma (ensures shiftn i (bracket_abstraction t) = bracket_abstraction (shiftn_lam i t))
         (decreases t)
 = match t with
-  | Abs a t ->
+  | Abs t ->
     shift_abs i (bracket_abstraction t) ;
     shift_bracket (i + 1) t
   | App t u -> shift_bracket i t ; shift_bracket i u
@@ -185,14 +168,14 @@ let rec shift_bracket (i : nat) (t : lam)
 let ski_eq_S_K (t u : ski)
 : ski_eq (App (App S (App K t)) (App K u)) (App K (App t u))
 = let ext (i : nat {not_free i t && not_free i u})
-  = let red_S = Red_S (App K t) (App K u) (Var i) in
-    let red_K_l = Red_K t (Var i) in
-    let red_K_r = Red_K u (Var i) in
-    let red_K_app = ski_app_eq (SStep red_K_l) (SStep red_K_r) in
-    let lhs = STran (SStep red_S) red_K_app in
-    let red_K = Red_K (App t u) (Var i) in
-    let rhs = SSymm (SStep red_K) in
-    STran lhs rhs
+  = let red_S = RedS (App K t) (App K u) (Var i) in
+    let red_K_l = RedK t (Var i) in
+    let red_K_r = RedK u (Var i) in
+    let red_K_app = app_eq_ski red_K_l red_K_r in
+    let lhs = Eq_S (Tran red_S red_K_app) in
+    let red_K = RedK (App t u) (Var i) in
+    let rhs = Eq_S (Symm red_K) in
+    Eq_S (Tran lhs rhs)
   in Zeta ext
 
 let rec ski_eq_abstract (t : ski)
@@ -201,23 +184,23 @@ let rec ski_eq_abstract (t : ski)
   | App t u ->
     let hi_t = ski_eq_abstract t in
     let hi_u = ski_eq_abstract u in
-    let hi_appl = SAppR S hi_t in
-    let hi_app = ski_app_eq hi_appl hi_u in
+    let hi_appl = Eq_S (AppR S hi_t) in
+    let hi_app = app_eq_ski hi_appl hi_u in
     let eq_SK = ski_eq_S_K t u in
-    STran hi_app eq_SK
-  | _ -> SRefl _
+    Eq_S (Tran hi_app eq_SK)
+  | _ -> Eq_S (Refl _)
 
 let rec subst_abstract (t : ski) (v : ski) (i : nat)
 : ski_eq (abstract (subst_ski t (shift_ski v) (i + 1)))
          (subst_ski (abstract t) v i)
 = match t with
   | App t u ->
-    ski_app_eq (SAppR S (subst_abstract t v i)) (subst_abstract u v i)  
+    app_eq_ski (Eq_S (AppR S (subst_abstract t v i))) (subst_abstract u v i)  
   | Var j ->
     if j = i + 1
     then ski_eq_abstract v
-    else SRefl _
-  | _ -> SRefl _
+    else Eq_S (Refl _)
+  | _ -> Eq_S (Refl _)
 
 
 let rec subst_bracket (t : lam) (v : lam) (i : nat)
@@ -225,28 +208,31 @@ let rec subst_bracket (t : lam) (v : lam) (i : nat)
               (subst_ski (bracket_abstraction t) (bracket_abstraction v) i))
       (decreases t)
 = match t with
-  | Abs _ t ->
+  | Abs t ->
     shift_bracket 0 v ;
     let hi = subst_bracket t (shift_lam v) (i + 1) in
     let hi = abstract_ski_eq hi in 
     let bracket_t = bracket_abstraction t in
     let bracket_v = bracket_abstraction v in
     let subst_abstract_eq = subst_abstract bracket_t bracket_v i in
-    STran hi subst_abstract_eq
-  | App t u -> ski_app_eq (subst_bracket t v i) (subst_bracket u v i)
-  | _ -> SRefl _
+    Eq_S (Tran hi subst_abstract_eq)
+  | App t u -> app_eq_ski (subst_bracket t v i) (subst_bracket u v i)
+  | _ -> Eq_S (Refl _)
 
 
-let rec step_preserves_eq (#t #u : lam) (st : step t u)
-: ski_eq (bracket_abstraction t) (bracket_abstraction u) =
-  match st with
-  | AppL st_t u -> 
-    SAppL (step_preserves_eq st_t) (bracket_abstraction u)
-  | AppR t st_u ->
-    SAppR (bracket_abstraction t) (step_preserves_eq st_u)
-  | Beta _ t u ->
+let rec bracket_preserves_eq (#t #u : lam) (r : lam_eq t u)
+: Tot (ski_eq (bracket_abstraction t) (bracket_abstraction u)) (decreases r) =
+  match r with
+  | Eq_L (Refl _) -> Eq_S (Refl _)
+  | Eq_L (Symm r) -> Eq_S (Symm (bracket_preserves_eq r))
+  | Eq_L (Tran r1 r2) -> Eq_S (Tran (bracket_preserves_eq r1) (bracket_preserves_eq r2))
+  | Eq_L (AppL r u) -> 
+    Eq_S (AppL (bracket_preserves_eq r) (bracket_abstraction u))
+  | Eq_L (AppR t r) ->
+    Eq_S (AppR (bracket_abstraction t) (bracket_preserves_eq r))
+  | Beta t u ->
     let bracket_t = bracket_abstraction t in
     let bracket_u = bracket_abstraction u in
-    STran (abstract_App bracket_t bracket_u) (SSymm (subst_bracket t u 0))
-  | Down _ st -> abstract_ski_eq (step_preserves_eq st)
+    Eq_S (Tran (abstract_App bracket_t bracket_u) (Eq_S (Symm (subst_bracket t u 0))))
+  | Down r -> abstract_ski_eq (bracket_preserves_eq r)
   
