TrLam.Equality.fst
@@ -1,0 +1,18 @@
+module TrLam.Equality
+
+open SKI
+open TrLam
+open SKI.Equality
+
+
+
+let rec trlam_preserves_eq (#t #u : ski) (r : ski_eq t u)
+: Tot (lam_eq (trlam t) (trlam u)) (decreases r)
+= match r with
+  | Eq_S (Refl _) -> Eq_L (Refl _)
+  | Eq_S (Symm r) -> Eq_L (Symm (trlam_preserves_eq r))
+  | Eq_S (Tran r1 r2) ->
+    Eq_L (Tran (trlam_preserves_eq r1)
+               (trlam_preserves_eq r2))
+  | RedI x -> admit ()
+  | _ -> admit ()
