TrLam.fst
@@ -1,0 +1,16 @@
+module TrLam
+
+open SKI
+
+let rec trlam (t : ski) : lam =
+  match t with
+  | Unit -> Unit
+  | Var i -> Var i
+  | S -> 
+    let f = Var 2 in
+    let g = Var 1 in
+    let x = Var 0 in
+    Abs (Abs (Abs (App (App f x) (App g x))))
+  | K -> Abs (Abs (Var 1))
+  | I -> Abs (Var 0)
+  | App t u -> App (trlam t) (trlam u)
